\documentclass{article}
\usepackage[margin=3cm]{geometry}
\usepackage[utf8]{inputenc}
\usepackage{amsmath}
\usepackage{amssymb}
\usepackage{float}
\usepackage{enumitem}
\usepackage{graphicx}
\usepackage{caption}
\usepackage{subcaption}
\usepackage{comment}
\usepackage{eurosym}

\graphicspath{ {plots/} }

\title{Dynamic Optimization - Homework assignment 9}
\author{Christian Segercrantz 481056}


\begin{document}
	\maketitle
	\pagebreak

\section*{9.4}

We know the state equation 
\begin{equation}
	\dot{x} = -10x(t) + u(t)
\end{equation}
and we want to minimize the performance measure
\begin{equation}
	J= \frac{1}{2}x^2(0.04) + \int_{0}^{0.04} \left[ \frac{1}{4}x^2(t) + \frac{1}{2}u^2(t) \right]  dt
\end{equation}
We will write the Hamiltonian as
\begin{equation}
	H(x,u,p,t) = \frac{1}{4}x^2(t) + \frac{1}{2}u^2(t) + \nabla_x J^* (t,x)(-10x(t) + u(t))
\end{equation}
The Hamilton-Jacobi-Bellman equation is
\begin{align}
	0 = \min_{u\in U}\left[ \nabla_t J^*(t,x) + H(x,u,p,t)\right].
\end{align}
We take the first order derivative of the Hamiltonian w.r.t $u$ and get
\begin{equation}
	H_u = u+\nabla_xJ^*,
\end{equation}
which we then minimize by setting the left hand side to 0. This gives us
\begin{align}
	0 =&  u^*+\nabla_xJ^* \\
	u^* =& - \nabla_xJ^* \\
	\implies H =&  \frac{1}{4}x^2 + \frac{1}{2}(- \nabla_xJ^*)^2 + \nabla_x J^*\cdot(-10x  - \nabla_xJ^*) \\
	=& \frac{1}{4}x^2 - \frac{1}{2}(\nabla_xJ^*)^2 -10x\nabla_x J^* \\
	\implies \text{ HJB: } 0 =& J_t^*(t,x) + \frac{1}{4}x^2 - \frac{1}{2}(J_x^*)^2 -10x J_x^*, \qquad | (-J_x^*)^2 = (J_x^*)^2
\end{align}
We will use the trial function and the following results
\begin{align}
	J(x(t),t) =& a(t)x^2(t) + b(t)x(t) + c(t) \\
	J_x =& 2ax + b \\
	J_t =& \dot{a}x^2 + \dot{b}x + \dot{c} \\
	u =& -2ax - b
\end{align}
By inserting this into the HJB equation we get
\begin{align}
	0 =& \dot{a}x^2 + \dot{b}x + \dot{c} + \frac{1}{4}x^2 - \frac{1}{2}(2ax + b) ^2 - 10x(2ax + b) \\
	-(\dot{a}x^2 + \dot{b}x + \dot{c})=& \frac{1}{4}x^2 -2 a^2 x^2 - 2 a b x - \frac{1}{2} b^2 - 20ax^2 + 10bx \\
	-(\dot{a}x^2 + \dot{b}x + \dot{c})=& x^2\left( \frac{1}{4}-2a^2 - 20a\right) +x(-2ab-10b) -\frac{1}{2}b^2
\end{align}
And by comparing the terms on both side we get the three DEs
\begin{align}
	-\dot{a} =& \frac{1}{4}-2a^2-20a \label{eq:1}\\
	-\dot{b} =& -2ab - 10b \label{eq:2}\\
	-\dot{c} =& -\frac{1}{2} b^2 \label{eq:3}
\end{align}
Additionally we know from the final state that 
\begin{align}
	a(0.04)x^2(0.04) + b(0.04)x(0.04) + c(0.04) =& \frac{1}{2}x^2(0.04)\\
	\iff &\\
	a(0.04) =& \frac{1}{2} \label{final_a}\\
	b(0.04) =& 0\label{final_b}\\
	c(0.04) =& 0\label{final_c}
\end{align}

We insert equations \ref{eq:1}-\ref{eq:3} into Mathematica (in the form seen below) to solve 
\begin{verbatim}
DSolve[{-a'[t] == 	1/4 - 2 a[t]^2 - 20 a[t],
        -b'[t] == -2 a[t]*b[t] - 	10 b[t],
        -c'[t] == -1/2 b[t]^2},
       {a, b, c}, t]
\end{verbatim}
and get the following results.
\begin{align}
 	a^* =& -\frac{\sqrt{402} e^{\sqrt{402} t+4 \sqrt{402} c_1}+20 e^{\sqrt{402} t+4 \sqrt{402} c_1}-\sqrt{402}+20}{4 \left(1+e^{\sqrt{402} t+4 \sqrt{402} c_1}\right)} \\
 	b^* =& c_2 \exp \left(-\sqrt{\frac{201}{2}} \left(-t+\sqrt{\frac{2}{201}} \log \left(1+e^{\sqrt{402} (t+4 c_1)}\right)\right)\right) \\
 	c^* =& c_3-\frac{e^{-4 \sqrt{402} c_1} c_2{}^2}{2 \sqrt{402} \left(1+e^{\sqrt{402} (t+4 c_1)}\right)}
\end{align}.

The optimal control law is then
\begin{align}
	u^* =& - \nabla_xJ^* = 2ax + b \\
	u^* =& \frac{x \left(\sqrt{402} e^{\sqrt{402} x+4 \sqrt{402} c_1}+20 e^{\sqrt{402} x+4 \sqrt{402} c_1}-\sqrt{402}+20\right)}{2 \left(1+e^{\sqrt{402} x+4 \sqrt{402} c_1}\right)}-\\ 
	&c_2 \exp \left(-\sqrt{\frac{201}{2}} \left(-x+\sqrt{\frac{2}{201}} \log \left(1+e^{\sqrt{402} (x+4 c_1)}\right)\right)\right)
\end{align}
Using Equations \ref{final_a}-\ref{final_c} we get the following for for the answers:
\begin{align}
	a^* =& -\frac{-2.40131+(40.0499\, -\text{4.904702795618173$\grave{ }$*${}^{\wedge}$-15} i) \left(-e^{\sqrt{402} t}\right)}{4 \left(48.0861\, -(1.\, -\text{1.2246467991473532$\grave{ }$*${}^{\wedge}$-16} i) e^{\sqrt{402} t}\right)}\\
	b^* =& 0\\
	c^* =& 0\\
	u^* =&  \frac{x \left(-2.40131+(40.0499\, -\text{4.904702795618173}\cdot10^{-15} i) \left(-e^{\sqrt{402} x}\right)\right)}{2 \left(48.0861\, -(1.\, -\text{1.2246467991473532}\cdot10^{-16} i) e^{\sqrt{402} x}\right)}\\
	\approx & \frac{\left(-40.0499 e^{\sqrt{402} x}-2.40131\right) x}{2 \left(48.0861\, -1. e^{\sqrt{402} x}\right)}
\end{align}
\end{document}




