\documentclass{article}
\usepackage[margin=3cm]{geometry}
\usepackage[utf8]{inputenc}
\usepackage{amsmath}
\usepackage{amssymb}
\usepackage{float}
\usepackage{enumitem}
\usepackage{graphicx}
\usepackage{caption}
\usepackage{subcaption}

\graphicspath{ {plots/} }

\title{Dynamic Optimization - Homework assignment 1}
\author{Christian Segercrantz 481056}


\begin{document}
	\maketitle
	\pagebreak

\section*{1.5}
\subsection*{a)}

We have the functional
\begin{equation}
	J(x,t) = \int_{0}^{T} \frac{\dot{x}^2}{t^3}dt
\end{equation}
with the end points $x(0) = A$ and $x(t) = B$.

To find the extremals fo the functional, we use Eulers equation
\begin{equation}
	g_x-\frac{d}{dt}g_{\dot{x}} = 0.
\end{equation}
where
\begin{align}
	g(x,\dot{x},t) = g &= \frac{\dot{x}^2}{t^3}\\
	\frac{\partial}{\partial x} g= g_x &=  0 \\
	\frac{\partial}{\partial \dot{x}} g= g_{\dot{x}} &=  \frac{2\dot{x}}{t^3}
\end{align}
which gives us the equation
\begin{equation}
	0 - \frac{d}{dt} \frac{2\dot{x}}{t^3} = 0.
\end{equation}
The derivative can be calculated as
\begin{equation}
	\frac{d}{dt} \frac{2\dot{x}}{t^3} 
	= \frac{\frac{d}{dt}(2\dot{x})t^3 - \frac{d}{dt}(t^3)2\dot{x}}{(t^3)^2}
	= \frac{2\ddot{x}t^3 - 6t^2\dot{x}}{t^6}
	= \frac{2\ddot{x}t - 6\dot{x}}{t^4}
\end{equation}
from which our already modified eulers equation becomes 
\begin{align}
	\frac{2\ddot{x}t - 6\dot{x}}{t^4} &= 0\\
	\frac{\ddot{x}}{t^3} - \frac{3\dot{x}}{t^4} &= 0\\
	\frac{\ddot{x}}{t^3} &= \frac{3\dot{x}}{t^4} \\
	\frac{\ddot{x}}{\dot{x}} &= \frac{3}{t}.
\end{align}
We can begin solving the ODE by integrating
\begin{align}
	\int\ddot{x} t dt &= \int3 \dot{x}dt\\
	t\dot{x} - \int \dot{x} dt &= 3 x + c\\
	t\dot{x} - x &= 3x +c\\
	t\dot{x} - 4x -c &= 0
\end{align}
which yields us the linear first order ODE which can be solved as 
\begin{align}
	\dot{x} - \frac{4}{t}x - \frac{c}{t} &= 0, \qquad |\cdot e^{P(x)},P(x) = \int-\frac{4}{t}dt = -4\ln(t)\\
	\dot{x}e^{-4\ln{t}} - \frac{4}{t}xe^{-4\ln{t}} - \frac{c}{t}e^{-4\ln{t}} &= 0, \qquad | e^{-4\ln{t}} = t^{-4}\\
	\frac{d}{dt}\left(xt^{-4}\right) &= \frac{c}{t}t^{-4} = ct^{-5}, \qquad |\int dt\\
	xt^{-4} &= -ct^{-4} +b, \qquad |\cdot t^4\\
	x &= -c +bt^4, \qquad c_1 = b, c_2 = -c \\
	x(t) &= c_1 t^4 + c_2.
\end{align}
We can solve the constants from the en point conditions: $x(0) = A$ and $x(t) = B$
\begin{align}
	x(0) &= c_1 0^4 + c_2  = A \implies c_2 = A\\
	x(T) &= c_1 T^4 + A = B \implies c_1 = \frac{B-A}{T^4} \\
	\implies x(t) &= \frac{B-A}{T^4} t^4 + A.
\end{align}

\subsection*{b)}
We have the functional
\begin{equation}
	J(x,t) = \int_{0}^{T} (\dot{x} - 8xt +t) dt
\end{equation}
with the end points $x(0) = A$ and $x(t) = B$.

To find the extremals fo the functional, we use Eulers equation
\begin{equation}
	g_x-\frac{d}{dt}g_{\dot{x}} = 0.
\end{equation}
where
\begin{align}
	g(x,\dot{x},t) = g &= \dot{x}^2 - 8xt +t\\
	\frac{\partial}{\partial x} g= g_x &=  -8t \\
	\frac{\partial}{\partial \dot{x}} g= g_{\dot{x}} &=  2\dot{x}
\end{align}
which gives us the equation
\begin{align}
	-8t - \frac{d}{dt} 2\dot{x} &= 0\\
	8t + 2\ddot{x} &= 0\\
	\ddot{x} &= -4t.
\end{align}
We can solve the DE by integrating twice
\begin{align}
	\int\ddot{x}dt &= \int -4t dt\\
	\dot{x} &= -2t^2 +c, \qquad |\int dt\\
	\int \dot{x} &= \int -2t^2 +c dt\\
	x &= -\frac{2}{3}t^3+ct+b, \qquad c_1 = c, c_2 = b
\end{align}
Solving the linear ODE we get the solution 
\begin{equation}
	x(t) = -\frac{2t^3}{3} + c_1 t + c_2.
\end{equation}
We can solve the constants from the en point conditions: $x(0) = A$ and $x(t) = B$
\begin{align}
	x(0) &= -\frac{2\cdot0^3}{3} + c_1 0 + c_2 = A \implies c_2 = A\\
	x(T) &= -\frac{2T^3}{3} + c_1 T + A = B \implies c_1 = \frac{B-A + \frac{2}{3}T^3}{T} \\
	\implies x(t) &= -\frac{2}{3}t^3 + \frac{B-A + \frac{2}{3}T^3}{T} t + A.
\end{align}
\end{document}




