\documentclass{article}
\usepackage[margin=3cm]{geometry}
\usepackage[utf8]{inputenc}
\usepackage{amsmath}
\usepackage{amssymb}
\usepackage{float}
\usepackage{enumitem}
\usepackage{graphicx}
\usepackage{caption}
\usepackage{subcaption}

\graphicspath{ {plots/} }

\title{Dynamic Optimization - Presentation exercise 1}
\author{Christian Segercrantz 481056}


\begin{document}
	\maketitle
	\pagebreak

\section*{1.1}
\subsection*{b)}
	
	\begin{align}
		g_{x_1} =& 2x_1 + x_2 \\
		g_{x_2} =& x_1+2x_2 \\
		g_{\dot{x}_1} =& 2x_2\\
		g_{\dot{x}_2} =& 2x_1
	\end{align}
	We use equation 10 from the lecture slides
	\begin{align}
		\delta J (x,\delta x) =& \int_{t_0}^{t_f}\left[g_{x_1}\delta x_1 + g_{x_2}\delta x_2 + g_{\dot{x}_1}\delta \dot{x}_1 + g_{\dot{x}_2}\delta \dot{x}_2 \right] dt
	\end{align}
	Integration by parts
	\begin{align}
		\int_{t_0}^{t_f} 2\dot{x}_1 \delta \dot{x}_2 dt = 2\left(\dot{x}_1(t_f)\underbrace{\delta x_1(t_f)}_{0}- \dot{x}_1(t_0) \underbrace{\delta x_2(t_0)}_{0} \right) - \int_{t_0}^{t_f} 2 \ddot{x}_1 \delta x_2 dt
	\end{align}
	Subsitution
	\begin{align}
		\delta J(x, \delta x) = & \int_{t_0}^{t_f} \left[ (2x_1+x_2) \delta x_1 + (x_1 +2x_2) \delta x_2 \right] dt - \int_{t_0}^{t_f} 2 \ddot{x}_2 \delta x_1  - \int_{t_0}^{t_f} 2 \ddot{x}_1 \delta x_2\\
		\delta J(x, \delta x) = & \int_{t_0}^{t_f} \left[ (2x_1+x_2) \delta x_1 + (x_1 +2x_2) \delta x_2 - 2\ddot{x}_2 \delta x_1 - 2 \ddot{x}_1 \delta x_2 \right] dt
	\end{align}
\pagebreak
\subsection*{c)}
	We use equation 10 from the lecture slides
	\begin{align}
		J(x) &= \int_{t_0}^{t_f} e^{x(t)}dt\\
		\delta J(x,\delta x) &= \int_{t_0}^{t_f} \left[ \frac{\partial g}{\partial x}\delta x + \underbrace{\frac{\partial g}{\partial \dot{x}}\delta \dot{x}}_{0}\right]\\
		\delta J(x,\delta x) &= \int_{t_0}^{t_f} \left[ \frac{\partial e^{x}}{\partial x}\delta x\right]	\\
		\delta J(x,\delta x) &= \int_{t_0}^{t_f}  e^{x}\delta x
	\end{align}

\pagebreak
\section*{1.3}
\subsection*{a)}
	\begin{equation}
		x^2+\dot{x}^2
	\end{equation}
	Eulers: 
	\begin{align}
		g_x - \frac{d}{dt} g_{\dot{x}} =& 0\\
		g_x =& 2x \\
		g_{\dot{x}} =& 2\dot{x} \\
		\implies 2x - \frac{d}{dt} 2\dot{x} =& 0\\
		2x - 2\ddot{x} &= 0\\
		x - \ddot{x} &= 0
	\end{align}
	We solve the DE by using the guess $x = e^{z t}$:
	\begin{align}
		x - \ddot{x} = 0 \implies e^{z t} - z^2 e^{z t} &= 0 \\
		e^{z t}(1 - z^2) &= 0\\
		1 - z^2 &= 0
	\end{align}
	General solution: $x(t) = c_1 e^{z_1 t} - c_2 e^{z_2 t}$
\pagebreak
\subsection*{b)}
 \begin{align}
 	J(x) &= \int^0_2 x^2 +2x\dot{x} + \dot{x}^2 dt, x(0) = 1, x(2) = -3\\
 	g_x &= 2x +2\dot{x}\\
 	g_{\dot{x}} &= 2x +2\dot{x}	
 \end{align}

	Eulers: 
	\begin{align}
		g_x - \frac{d}{dt} g_{\dot{x}} =& 0\\
		2x +2\dot{x} - \frac{d}{dt}2x +2\dot{x}	 &= 0\\
		2x +2\dot{x} - 2\dot{x} +2\ddot{x} &= 0\\
		2x +2\ddot{x} &= 0 \iff x +\ddot{x} = 0
	\end{align}
	Same as in the pervious exercise: \\
	We solve the DE by using the guess $x = e^{z t}$:
	\begin{align}
		x - \ddot{x} = 0 \implies e^{z t} - z^2 e^{z t} &= 0 \\
		e^{z t}(1 - z^2) &= 0\\
		1 - z^2 &= 0\\
		z &= \pm 1
	\end{align}
	General solution: $x(t) = c_1 e^{z_1 t} + c_2 e^{z_2 t}$ and using the roots we get the solution below. By thend point 
	\begin{align}
		x &= c_1 e^{t} + c_2 e^{- t}\\
		x(0) &= c_1 e^0 + c_2 e^{0} = c_1 + c_2 = 1 \iff c_1 = 1 - c_2\\
		x(2) &= c_1 e^{2} + c_2 e^{-2} = (1-c_2)e^{2} + c_2 e^{-2} \\
		&= e^{2}-c_2e^{2} + c_2 e^{-2}\\
		&= c_2(-e^{2} + e^{-2}) +e^{2} = -3\\
		c_2(-e^{2} + e^{-2}) &= -3 - e^{2}\\
		c_2 &= \frac{-3 - e^{2}}{-e^{2} + e^{-2}} = -\frac{3 + e^{2}}{e^{-2} -e^{2}}\\
		\implies c_1 &= 1 + \frac{3 + e^{2}}{e^{-2} -e^{2}} = \frac{e^{-2} -e^{2} + 3 + e^{2}}{e^{-2} -e^{2}}\\
		\implies x &= \frac{e^{-2} -e^{2} + 3 + e^{2}}{e^{-2} -e^{2}} e^{t} -\frac{3 + e^{2}}{e^{-2} -e^{2}} e^{- t}\\
		%x &= \frac{\left(e^{-2} -e^{2} + 3 + e^{2}\right)e^{t}-\left(3 + e^{2}\right)e^{- t}}{e^{-2} -e^{2}} | \cdot -e^2 \\
		%x &= \frac{\left(-e^{4} + 3e^{2} + e^{4}\right)e^{t}-\left(3e^{2} + e^{4}\right)e^{- 2t}}{e^{4} -1}\\
	\end{align}
\end{document}